@prefix dc: <http://purl.org/dc/elements/1.1/> .
@prefix dcterms: <http://purl.org/dc/terms/> .
@prefix eop: <http://www.opengis.net/ont/eo-geojson/1.0/> .
@prefix ianarel: <http://www.iana.org/assignments/relation/> .
@prefix media: <http://search.yahoo.com/mrss/> .
@prefix owc: <http://www.opengis.net/ont/owc/1.0/> .
@prefix owl: <http://www.w3.org/2002/07/owl#> .
@prefix rdf: <http://www.w3.org/1999/02/22-rdf-syntax-ns#> .
@prefix rdfs: <http://www.w3.org/2000/01/rdf-schema#> .
@prefix skos: <http://www.w3.org/2004/02/skos/core#> .
@prefix vann: <http://purl.org/vocab/vann/> .
@prefix void: <http://rdfs.org/ns/void#> .
@prefix xml: <http://www.w3.org/XML/1998/namespace> .
@prefix xsd: <http://www.w3.org/2001/XMLSchema#> .

media:category a owl:ObjectProperty ;
    rdfs:label "category" ;
    dc:description """Media category of the related resource which corresponds to a preview or mask:
- THUMBNAIL
- QUICKLOOK
- ALBUM
- SNOW
- CLOUD
- QUALITY
Only applicable for media resources.""";
    dcterms:source "OGC 17-003, MediaRSS"^^xsd:string ;
    rdfs:isDefinedBy media: ;
    rdfs:seeAlso <http://www.rssboard.org/media-rss#media-category> .

media:expression a owl:DatatypeProperty ;
    rdfs:label "expression" ;
    dc:description "Determines if the related resource is a sample or the full version of the product.  Use \"full\" for “product/ProductInformation/”.  Use \"sample\" for \"browse/BrowseInformation/\" or \"mask/MaskInformation/\"." ;
    dcterms:source "OGC 17-003, MediaRSS"^^xsd:string ;
    rdfs:isDefinedBy media: ;
    rdfs:seeAlso <http://www.rssboard.org/media-rss#media-content> .

ianarel:describedby a owl:ObjectProperty ;
    rdfs:label "qualityReport" ;
    dc:description "Reference to the location of a related quality report as defined by OGC 14-055r2 §7.1.2." ;
    dcterms:source "OGC 17-003, OGC 14-055r2"^^xsd:string ;
    rdfs:isDefinedBy eop: ;
    rdfs:seeAlso <https://tools.ietf.org/html/rfc5988> .

ianarel:related a owl:ObjectProperty ;
    rdfs:label "related" ;
    dc:description "Reference to the location of a related resource, e.g. cloud mask, snow mask." ;
    dcterms:source "OGC 17-003"^^xsd:string ;
    rdfs:isDefinedBy eop: ;
    rdfs:seeAlso <https://tools.ietf.org/html/rfc5988> .

ianarel:up a owl:ObjectProperty ;
    rdfs:label "up" ;
    dc:description "Reference to the metadata of higher level resource (e.g.  Collection, also identified by parentIdentifier) resource." ;
    dcterms:source "OGC 17-003"^^xsd:string ;
    rdfs:isDefinedBy eop: ;
    rdfs:seeAlso <https://tools.ietf.org/html/rfc5988> .

eop:ABSORPTION a eop:MeasurementType ;
    dc:description "Measurement type constant." .

eop:ACQUIRED a eop:StatusType ;
    dc:description "Acquisition status constant." .

eop:ALBUM a eop:CategoryType ;
    dc:description "Category constant." .

eop:ALTIMETRIC a eop:SensorType ;
    dc:description "Sensor type constant." .

eop:ARCHIVED a eop:StatusType ;
    dc:description "Acquisition status constant." .

eop:ASCENDING a eop:OrbitDirectionType ;
    dc:description "Orbit direction constant." .

eop:ATMOSPHERIC a eop:SensorType ;
    dc:description "Sensor type constant." .

<http://www.opengis.net/ont/eo-geojson/1.0/AcquisitionType/CALIBRATION> a eop:AcquisitionType ;
    dc:description "Acquisition type constant." .

<http://www.opengis.net/ont/eo-geojson/1.0/AcquisitionType/NOMINAL> a eop:AcquisitionType ;
    dc:description "Acquisition type constant." .

<http://www.opengis.net/ont/eo-geojson/1.0/AcquisitionType/OTHER> a eop:AcquisitionType ;
    dc:description "Acquisition type constant." .

eop:CANCELLED a eop:StatusType ;
    dc:description "Acquisition status constant." .

eop:CLOUD a eop:CategoryType ;
    dc:description "Category constant." .

eop:DESCENDING a eop:OrbitDirectionType ;
    dc:description "Orbit direction constant." .

eop:EMISSION a eop:MeasurementType ;
    dc:description "Measurement type constant." .

eop:EarthObservation a owl:Class ;
    rdfs:label "EarthObservation" ;
    vann:example """
{
    "@context": "https://www.opengis.net/eo-geojson/1.0",
    "type": "Feature",
    "id": http://fedeo.esa.int/opensearch/request/?parentIdentifier=SEA_GEC_1P&uid=SE1_OPER_SEA_GEC_1P_19780927T010430_19780927T010445_001316_0000_2267_9B4F",
    "bbox": [
        -2.69574,
        61.965195,
        0.135472,
        63.261372
    ],
    "geometry": {...},
    "properties": {...}
}
  """;
    rdfs:comment " Earth Observation as defined in OGC 10-157r4" ;
    rdfs:isDefinedBy eop: ;
    rdfs:subClassOf <http://purl.org/geojson/vocab#Feature> .

eop:FAILED a eop:StatusType ;
    dc:description "Acquisition status constant." .

eop:GEO a eop:OrbitType ;
    dc:description "Orbit type constant." .

eop:LEFT a eop:AntennaLookDirectionType ;
    dc:description "Antenna look direction constant." .

eop:LEO a eop:OrbitType ;
    dc:description "Orbit type constant." .

eop:LIMB a eop:SensorType ;
    dc:description "Sensor type constant." .

eop:OPTICAL a eop:SensorType ;
    dc:description "Sensor type constant." .

eop:PLANNED a eop:StatusType ;
    dc:description "Acquisition status constant." .

eop:POTENTIAL a eop:StatusType ;
    dc:description "Acquisition status constant." .

<http://www.opengis.net/ont/eo-geojson/1.0/PolarisationChannels/HH> a eop:PolarisationChannelsType ;
    dc:description "Polarisation channel constant." .

<http://www.opengis.net/ont/eo-geojson/1.0/PolarisationChannels/HH_HV> a eop:PolarisationChannelsType ;
    dc:description "Polarisation channel constant." .

<http://www.opengis.net/ont/eo-geojson/1.0/PolarisationChannels/HH_HV_VH_VV> a eop:PolarisationChannelsType ;
    dc:description "Polarisation channel constant." .

<http://www.opengis.net/ont/eo-geojson/1.0/PolarisationChannels/HH_VH> a eop:PolarisationChannelsType ;
    dc:description "Polarisation channel constant." .

<http://www.opengis.net/ont/eo-geojson/1.0/PolarisationChannels/HH_VV> a eop:PolarisationChannelsType ;
    dc:description "Polarisation channel constant." .

<http://www.opengis.net/ont/eo-geojson/1.0/PolarisationChannels/HV> a eop:PolarisationChannelsType ;
    dc:description "Polarisation channel constant." .

<http://www.opengis.net/ont/eo-geojson/1.0/PolarisationChannels/HV_VH> a eop:PolarisationChannelsType ;
    dc:description "Polarisation channel constant." .

<http://www.opengis.net/ont/eo-geojson/1.0/PolarisationChannels/UNDEFINED> a eop:PolarisationChannelsType ;
    dc:description "Polarisation channel constant." .

<http://www.opengis.net/ont/eo-geojson/1.0/PolarisationChannels/VH> a eop:PolarisationChannelsType ;
    dc:description "Polarisation channel constant." .

<http://www.opengis.net/ont/eo-geojson/1.0/PolarisationChannels/VH_HV> a eop:PolarisationChannelsType ;
    dc:description "Polarisation channel constant." .

<http://www.opengis.net/ont/eo-geojson/1.0/PolarisationChannels/VH_VV> a eop:PolarisationChannelsType ;
    dc:description "Polarisation channel constant." .

<http://www.opengis.net/ont/eo-geojson/1.0/PolarisationChannels/VV> a eop:PolarisationChannelsType ;
    dc:description "Polarisation channel constant." .

<http://www.opengis.net/ont/eo-geojson/1.0/PolarisationChannels/VV_HV> a eop:PolarisationChannelsType ;
    dc:description "Polarisation channel constant." .

<http://www.opengis.net/ont/eo-geojson/1.0/PolarisationChannels/VV_VH> a eop:PolarisationChannelsType ;
    dc:description "Polarisation channel constant." .

<http://www.opengis.net/ont/eo-geojson/1.0/PolarisationMode/D> a eop:PolarisationModeType ;
    dc:description "Polarisation mode constant." .

<http://www.opengis.net/ont/eo-geojson/1.0/PolarisationMode/Q> a eop:PolarisationModeType ;
    dc:description "Polarisation mode constant." .

<http://www.opengis.net/ont/eo-geojson/1.0/PolarisationMode/S> a eop:PolarisationModeType ;
    dc:description "Polarisation mode constant." .

<http://www.opengis.net/ont/eo-geojson/1.0/PolarisationMode/T> a eop:PolarisationModeType ;
    dc:description "Polarisation mode constant." .

<http://www.opengis.net/ont/eo-geojson/1.0/PolarisationMode/UNDEFINED> a eop:PolarisationModeType ;
    dc:description "Polarisation mode constant." .

eop:QUALITY a eop:CategoryType ;
    dc:description "Category constant." .

eop:QUALITYDEGRADED a eop:StatusType ;
    dc:description "Acquisition status constant." .

eop:QUICKLOOK a eop:CategoryType ;
    dc:description "Category constant." .

eop:RADAR a eop:SensorType ;
    dc:description "Sensor type constant." .

eop:REJECTED a eop:StatusType ;
    dc:description "Acquisition status constant." .

eop:RIGHT a eop:AntennaLookDirectionType ;
    dc:description "Antenna look direction constant." .

eop:SNOW a eop:CategoryType ;
    dc:description "Category constant." .

<http://www.opengis.net/ont/eo-geojson/1.0/SpectralRange/MICROWAVE> a eop:SpectralRangeType ;
    dc:description "SpectralRange type constant." .

<http://www.opengis.net/ont/eo-geojson/1.0/SpectralRange/OTHER> a eop:SpectralRangeType ;
    dc:description "SpectralRange type constant." .

<http://www.opengis.net/ont/eo-geojson/1.0/SpectralRange/UV> a eop:SpectralRangeType ;
    dc:description "SpectralRange type constant for Ultraviolet (UV)." .

<http://www.opengis.net/ont/eo-geojson/1.0/SpectralRange/VISIBLE> a eop:SpectralRangeType ;
    dc:description "SpectralRange type constant." .

eop:THUMBNAIL a eop:CategoryType ;
    dc:description "Category constant." .

eop:acquisitionAngles a owl:FunctionalProperty,
        owl:ObjectProperty ;
    rdfs:label "acquisitionAngles" ;
    dcterms:source "OGC 17-003"^^xsd:string ;
    rdfs:comment "Acquisition angles." ;
    rdfs:domain eop:AcquisitionParameters ;
    rdfs:isDefinedBy eop: ;
    rdfs:range eop:AcquisitionAngles .

eop:acquisitionInformation a owl:ObjectProperty ;
    rdfs:label "acquisitionInformation" ;
    dc:description "Contains acquisition information." ;
    dcterms:source "OGC 17-003"^^xsd:string ;
    rdfs:comment "Contains acquisition information." ;
    rdfs:domain eop:Properties ;
    rdfs:isDefinedBy eop: ;
    rdfs:range eop:AcquisitionInformation .

eop:acquisitionParameters a owl:FunctionalProperty,
        owl:ObjectProperty ;
    rdfs:label "acquisitionParameters" ;
    dc:description "The acquisition parameters (i.e. pointing angles, etc.)." ;
    dcterms:source "OGC 17-003"^^xsd:string ;
    rdfs:domain eop:AcquisitionInformation ;
    rdfs:isDefinedBy eop: ;
    rdfs:range eop:AcquisitionParameters .

eop:acquisitionStation a owl:DatatypeProperty ;
    rdfs:label "acquisitionStation" ;
    dcterms:source "OGC 17-003"^^xsd:string ;
    rdfs:comment "Acquisition / receiving station code. Possible values are mission specific and should be retrieved using codespace." ;
    rdfs:domain eop:AcquisitionParameters ;
    rdfs:isDefinedBy eop: ;
    rdfs:range xsd:string .

eop:acquisitionSubType a owl:DatatypeProperty ;
    rdfs:label "acquisitionSubType" ;
    dcterms:source "OGC 17-003"^^xsd:string ;
    rdfs:comment "The broad value defined by the acquisitionType is too restrictive, so mission specific type definition should refer to mission/ground segment dedicated codeSpace." ;
    rdfs:domain eop:AcquisitionParameters ;
    rdfs:isDefinedBy eop: ;
    rdfs:range xsd:string .

eop:acquisitionType a owl:FunctionalProperty,
        owl:ObjectProperty ;
    rdfs:label "acquisitionType" ;
    dc:description """AcquisitionType can be one of: 
 - NOMINAL
 - CALIBRATION
 - OTHER.""";
    dcterms:source "OGC 17-003"^^xsd:string ;
    rdfs:domain eop:AcquisitionParameters ;
    rdfs:isDefinedBy eop: ;
    rdfs:range eop:AcquisitionType .

eop:acrossTrackIncidenceAngle a owl:DatatypeProperty ;
    rdfs:label "acrossTrackIncidenceAngle" ;
    dcterms:source "OGC 17-003"^^xsd:string ;
    rdfs:comment "Acquisition across track incidence angle in degrees (i.e. uom='deg')." ;
    rdfs:domain eop:AcquisitionAngles ;
    rdfs:isDefinedBy eop: ;
    rdfs:range xsd:double .

eop:additionalAttributes a owl:ObjectProperty ;
    rdfs:label "additionalAttributes" ;
    dcterms:source "OGC 17-003"^^xsd:string ;
    rdfs:comment "Container for ad-hoc additional metadata attributes which are organisation or mission specific." ;
    rdfs:domain eop:DataIdentification ;
    rdfs:isDefinedBy eop: .

eop:alongTrackIncidenceAngle a owl:DatatypeProperty ;
    rdfs:label "alongTrackIncidenceAngle" ;
    dcterms:source "OGC 17-003"^^xsd:string ;
    rdfs:comment "Acquisition along track incidence angle in degrees (i.e. uom='deg')." ;
    rdfs:domain eop:AcquisitionAngles ;
    rdfs:isDefinedBy eop: ;
    rdfs:range xsd:double .

eop:altitudeUnit a owl:ObjectProperty ;
    rdfs:label "locationUnit" ;
    dcterms:source "OGC 17-003"^^xsd:string ;
    rdfs:comment "Unit of measure used to express lowestLocation and highestLocation: meter (m) or bar (bar). Default is meter (m)." ;
    rdfs:domain eop:VerticalSpatialDomain ;
    rdfs:isDefinedBy eop: ;
    rdfs:range eop:AltitudeUnitType .

eop:antennaLookDirection a owl:ObjectProperty ;
    rdfs:label "antennaLookDirection" ;
    dcterms:source "OGC 17-003"^^xsd:string ;
    rdfs:comment """Look direction of antenna taken from codelist
Values:
- LEFT
- RIGHT.""";
    rdfs:domain eop:AcquisitionParameters ;
    rdfs:isDefinedBy eop: ;
    rdfs:range eop:AntennaLookDirectionType .

eop:archivingCenter a owl:DatatypeProperty ;
    rdfs:label "archivingCenter" ;
    dcterms:source "OGC 17-003"^^xsd:string ;
    rdfs:comment "Archiving center code. Possible values are mission specific." ;
    rdfs:domain eop:ProductInformation ;
    rdfs:isDefinedBy eop: ;
    rdfs:range xsd:string .

eop:archivingDate a owl:DatatypeProperty ;
    rdfs:label "archivingDate" ;
    dcterms:source "OGC 17-003"^^xsd:string ;
    rdfs:comment "Archiving date time." ;
    rdfs:domain eop:ProductInformation ;
    rdfs:isDefinedBy eop: ;
    rdfs:range xsd:dateTime .

eop:ascendingNodeDate a owl:DatatypeProperty ;
    rdfs:label "ascendingNodeDate" ;
    dcterms:source "OGC 17-003"^^xsd:string ;
    rdfs:comment "UTC date and time at ascending node of orbit." ;
    rdfs:domain eop:OrbitParameters ;
    rdfs:isDefinedBy eop: ;
    rdfs:range xsd:dateTime .

eop:ascendingNodeLongitude a owl:DatatypeProperty ;
    rdfs:label "ascendingNodeLongitude" ;
    dcterms:source "OGC 17-003"^^xsd:string ;
    rdfs:comment """Longitude at ascending node of orbit. Should be expressed in degrees.
""";
    rdfs:domain eop:OrbitParameters ;
    rdfs:isDefinedBy eop: ;
    rdfs:range xsd:double .

eop:availabilityTime a owl:DatatypeProperty ;
    rdfs:label "availabilityTime" ;
    dcterms:source "OGC 17-003"^^xsd:string ;
    rdfs:comment """The time when the result becomes available
 dateTime in ISO 8601 format (CCYY-MM-DDThh:mm[:ss[.cc]]Z).""";
    rdfs:domain eop:ProductInformation ;
    rdfs:isDefinedBy eop: ;
    rdfs:range xsd:dateTime .

eop:cloudCover a owl:DatatypeProperty ;
    rdfs:label "cloudCover" ;
    dcterms:source "OGC 17-003"^^xsd:string ;
    rdfs:comment "Cloud cover percentage (i.e. uom=’%’)." ;
    rdfs:domain eop:CoverageDescription ;
    rdfs:isDefinedBy eop: ;
    rdfs:range xsd:double .

eop:completionTimeFromAscendingNode a owl:DatatypeProperty ;
    rdfs:label "completionTimeFromAscendingNode" ;
    dcterms:source "OGC 17-003"^^xsd:string ;
    rdfs:comment "Stop time of acquisition in milliseconds from ascending node date." ;
    rdfs:domain eop:AcquisitionParameters ;
    rdfs:isDefinedBy eop: ;
    rdfs:range xsd:integer .

eop:compositeType a owl:DatatypeProperty ;
    rdfs:label "compositeType" ;
    dcterms:source "OGC 17-003"^^xsd:string ;
    rdfs:comment "Type of composite product expressed as timeperiod that the composite product covers using ISO 8601 duration format P[n]Y[n]M[n]D encoding , e.g. P10D for a 10 day composite." ;
    rdfs:domain eop:ProcessingInformation ;
    rdfs:isDefinedBy eop: ;
    rdfs:range xsd:string ;
    rdfs:seeAlso <https://en.wikipedia.org/wiki/ISO_8601#Durations> .

eop:cycleNumber a owl:DatatypeProperty ;
    rdfs:label "cycleNumber" ;
    dcterms:source "OGC 17-003"^^xsd:string ;
    rdfs:comment "Number of Cycles." ;
    rdfs:domain eop:AcquisitionParameters ;
    rdfs:isDefinedBy eop: ;
    rdfs:range xsd:integer .

eop:discreteWavelength a owl:DatatypeProperty ;
    rdfs:label "discreteWavelengths" ;
    dcterms:source "OGC 17-003"^^xsd:string ;
    rdfs:comment "Discrete wavelength observed in the product.   Unit of measure is SI base unit (m) without prefix." ;
    rdfs:domain eop:WavelengthInformation ;
    rdfs:isDefinedBy eop: ;
    rdfs:range xsd:double .

eop:doi a owl:DatatypeProperty ;
    rdfs:label "doi" ;
    dcterms:source "OGC 17-003"^^xsd:string ;
    rdfs:comment "Digital Object Identifier identifying the product (see http://www.doi.org)." ;
    rdfs:domain eop:DataIdentification ;
    rdfs:isDefinedBy eop: ;
    rdfs:range xsd:string .

eop:dopplerFrequency a owl:DatatypeProperty ;
    rdfs:label "dopplerFrequency" ;
    dcterms:source "OGC 17-003"^^xsd:string ;
    rdfs:comment "Doppler Frequency of acquisition.   Unit of measure is SI base unit (m) without prefix." ;
    rdfs:domain eop:AcquisitionParameters ;
    rdfs:isDefinedBy eop: ;
    rdfs:range xsd:double .

eop:endWavelength a owl:DatatypeProperty ;
    rdfs:label "endWavelength" ;
    dcterms:source "OGC 17-003"^^xsd:string ;
    rdfs:comment "End of the observed wavelength range.  Unit of measure is SI base unit (m) without prefix." ;
    rdfs:domain eop:WavelengthInformation ;
    rdfs:isDefinedBy eop: ;
    rdfs:range xsd:double .

eop:groundTrackUncertainty a owl:DatatypeProperty ;
    rdfs:label "groundTrackUncertainty" ;
    dcterms:source "OGC 17-003"^^xsd:string ;
    rdfs:comment "Measure of the uncertainty of the ground track. Sometimes known as deadband e.g. 1000m (1Km) deadband.  Unit of measure is SI base unit (m) without prefix." ;
    rdfs:domain eop:AcquisitionParameters ;
    rdfs:isDefinedBy eop: ;
    rdfs:range xsd:double .

eop:illuminationAzimuthAngle a owl:DatatypeProperty ;
    rdfs:label "illuminationAzimuthAngle" ;
    dcterms:source "OGC 17-003"^^xsd:string ;
    rdfs:comment "Mean illumination/solar azimuth angle given in degrees (i.e. uom='deg')." ;
    rdfs:domain eop:AcquisitionAngles ;
    rdfs:isDefinedBy eop: ;
    rdfs:range xsd:double .

eop:illuminationElevationAngle a owl:DatatypeProperty ;
    rdfs:label "illuminationElevationAngle" ;
    dcterms:source "OGC 17-003"^^xsd:string ;
    rdfs:comment "Mean illumination/solar elevation angle in degrees (i.e. uom='deg')." ;
    rdfs:domain eop:AcquisitionAngles ;
    rdfs:isDefinedBy eop: ;
    rdfs:range xsd:double .

eop:illuminationZenithAngle a owl:DatatypeProperty ;
    rdfs:label "illuminationZenithAngle" ;
    dcterms:source "OGC 17-003"^^xsd:string ;
    rdfs:comment "Mean illumination/solar zenith angle in degrees (i.e. uom='deg')." ;
    rdfs:domain eop:AcquisitionAngles ;
    rdfs:isDefinedBy eop: ;
    rdfs:range xsd:double .

eop:incidenceAngle a owl:DatatypeProperty ;
    rdfs:label "incidenceAngle" ;
    dcterms:source "OGC 17-003"^^xsd:string ;
    rdfs:comment "Acquisition global incidence angle in degrees (i.e. uom='deg')." ;
    rdfs:domain eop:AcquisitionAngles ;
    rdfs:isDefinedBy eop: ;
    rdfs:range xsd:double .

eop:incidenceAngleVariation a owl:DatatypeProperty ;
    rdfs:label "incidenceAngleVariation" ;
    dcterms:source "OGC 17-003"^^xsd:string ;
    rdfs:comment "Incidence angle variation in degrees (i.e. uom='deg')." ;
    rdfs:domain eop:AcquisitionAngles ;
    rdfs:isDefinedBy eop: ;
    rdfs:range xsd:double .

eop:instrument a owl:FunctionalProperty,
        owl:ObjectProperty ;
    rdfs:label "instrument" ;
    dc:description """The Instrument/Sensor used for the acquisition.
If more than one instrument is used for creating the product, then the AcquisitionInformation object occurs more than once.""";
    dcterms:source "OGC 17-003"^^xsd:string ;
    rdfs:domain eop:AcquisitionInformation ;
    rdfs:isDefinedBy eop: ;
    rdfs:range eop:Instrument .

eop:instrumentAzimuthAngle a owl:DatatypeProperty ;
    rdfs:label "instrumentAzimuthAngle" ;
    dcterms:source "OGC 17-003"^^xsd:string ;
    rdfs:comment "Mean instrument azimuth angle in degrees (i.e. uom='deg')." ;
    rdfs:domain eop:AcquisitionAngles ;
    rdfs:isDefinedBy eop: ;
    rdfs:range xsd:double .

eop:instrumentElevationAngle a owl:DatatypeProperty ;
    rdfs:label "instrumentElevationAngle" ;
    dcterms:source "OGC 17-003"^^xsd:string ;
    rdfs:comment "Mean instrument elevation angle in degrees (i.e. uom='deg')." ;
    rdfs:domain eop:AcquisitionAngles ;
    rdfs:isDefinedBy eop: ;
    rdfs:range xsd:double .

eop:instrumentShortName a owl:DatatypeProperty ;
    rdfs:label "instrumentShortName" ;
    dcterms:source "OGC 17-003"^^xsd:string ;
    rdfs:comment "Instrument (Sensor) name." ;
    rdfs:domain eop:Instrument ;
    rdfs:isDefinedBy eop: ;
    rdfs:range xsd:string .

eop:instrumentZenithAngle a owl:DatatypeProperty ;
    rdfs:label "instrumentZenithAngle" ;
    dcterms:source "OGC 17-003"^^xsd:string ;
    rdfs:comment "Mean instrument zenith angle in degrees (i.e. uom='deg')." ;
    rdfs:domain eop:AcquisitionAngles ;
    rdfs:isDefinedBy eop: ;
    rdfs:range xsd:double .

eop:lastOrbitDirection a owl:ObjectProperty ;
    rdfs:label "lastOrbitDirection" ;
    dcterms:source "OGC 17-003"^^xsd:string ;
    rdfs:comment """Acquisition orbit direction at the end of the acquisition/product. Assumed to be identical to orbitDirection if not present.
Values:
•	ASCENDING
•	DESCENDING""";
    rdfs:domain eop:OrbitParameters ;
    rdfs:isDefinedBy eop: ;
    rdfs:range eop:OrbitDirectionType .

eop:lastOrbitNumber a owl:DatatypeProperty ;
    rdfs:label "lastOrbitNumber" ;
    dcterms:source "OGC 17-003"^^xsd:string ;
    rdfs:comment "Acquisition last orbit number." ;
    rdfs:domain eop:OrbitParameters ;
    rdfs:isDefinedBy eop: ;
    rdfs:range xsd:integer .

eop:maximumAltitude a owl:DatatypeProperty ;
    rdfs:label "highestLocation" ;
    dcterms:source "OGC 17-003"^^xsd:string ;
    rdfs:comment "Lower bound of measurements in vertical dimension.   Unit of measure defined by locationUnit property." ;
    rdfs:domain eop:VerticalSpatialDomain ;
    rdfs:isDefinedBy eop: ;
    rdfs:range xsd:double .

eop:maximumIncidenceAngle a owl:DatatypeProperty ;
    rdfs:label "maximumIncidenceAngle" ;
    dcterms:source "OGC 17-003"^^xsd:string ;
    rdfs:comment "Maximum incidence angle in degrees (i.e. uom='deg')." ;
    rdfs:domain eop:AcquisitionAngles ;
    rdfs:isDefinedBy eop: ;
    rdfs:range xsd:double .

eop:measurementType a owl:ObjectProperty ;
    rdfs:label "measurementType" ;
    dcterms:source "OGC 17-003"^^xsd:string ;
    rdfs:comment """Measurement type taken from codelist:
Values:
- ABSORPTION
- EMISSION.""";
    rdfs:domain eop:AcquisitionParameters ;
    rdfs:isDefinedBy eop: ;
    rdfs:range eop:MeasurementType .

eop:minimumAltitude a owl:DatatypeProperty ;
    rdfs:label "lowestLocation" ;
    dcterms:source "OGC 17-003"^^xsd:string ;
    rdfs:comment "Upper bound of measurements in vertical dimension.  Unit of measure defined by locationUnit property." ;
    rdfs:domain eop:VerticalSpatialDomain ;
    rdfs:isDefinedBy eop: ;
    rdfs:range xsd:double .

eop:minimumIncidenceAngle a owl:DatatypeProperty ;
    rdfs:label "minimumIncidenceAngle" ;
    dcterms:source "OGC 17-003"^^xsd:string ;
    rdfs:comment "Minimum incidence angle in degrees (i.e. uom='deg')." ;
    rdfs:domain eop:AcquisitionAngles ;
    rdfs:isDefinedBy eop: ;
    rdfs:range xsd:double .

eop:operationalMode a owl:DatatypeProperty ;
    rdfs:label "operationalMode" ;
    dcterms:source "OGC 17-003"^^xsd:string ;
    rdfs:comment "Sensor mode. Possible values are mission specific." ;
    rdfs:domain eop:AcquisitionParameters ;
    rdfs:isDefinedBy eop: ;
    rdfs:range xsd:string .

eop:orbitDirection a owl:ObjectProperty ;
    rdfs:label "orbitDirection" ;
    dcterms:source "OGC 17-003"^^xsd:string ;
    rdfs:comment """Acquisition orbit direction at the start of the acquisition/product.
Values:
•	ASCENDING
•	DESCENDING""";
    rdfs:domain eop:OrbitParameters ;
    rdfs:isDefinedBy eop: ;
    rdfs:range eop:OrbitDirectionType .

eop:orbitDuration a owl:DatatypeProperty ;
    rdfs:label "orbitDuration" ;
    dcterms:source "OGC 17-003"^^xsd:string ;
    rdfs:comment "Actual orbit duration in milliseconds." ;
    rdfs:domain eop:OrbitParameters ;
    rdfs:isDefinedBy eop: ;
    rdfs:range xsd:integer .

eop:orbitNumber a owl:DatatypeProperty ;
    rdfs:label "orbitNumber" ;
    dcterms:source "OGC 17-003"^^xsd:string ;
    rdfs:comment "Acquisition orbit number." ;
    rdfs:domain eop:OrbitParameters ;
    rdfs:isDefinedBy eop: ;
    rdfs:range xsd:integer .

eop:orbitType a owl:ObjectProperty ;
    rdfs:label "orbitType" ;
    dcterms:source "OGC 17-003"^^xsd:string ;
    rdfs:comment "High level characterisation of main mission types taken from a codelist." ;
    rdfs:domain eop:Platform ;
    rdfs:isDefinedBy eop: ;
    rdfs:range eop:OrbitType .

eop:parentIdentifier a owl:DatatypeProperty ;
    rdfs:label "parentIdentifier" ;
    dcterms:source "OGC 17-003"^^xsd:string ;
    vann:example """
{
    "parentIdentifier": "SEA_GEC_1P"
}
   """;
    rdfs:comment "Collection identifier." ;
    rdfs:domain eop:DataIdentification ;
    rdfs:isDefinedBy eop: ;
    rdfs:range xsd:string .

eop:pitch a owl:DatatypeProperty ;
    rdfs:label "pitch" ;
    dcterms:source "OGC 17-003"^^xsd:string ;
    rdfs:comment "Satellite pitch angle in degrees (i.e. uom='deg')." ;
    rdfs:domain eop:AcquisitionAngles ;
    rdfs:isDefinedBy eop: ;
    rdfs:range xsd:double .

eop:platform a owl:FunctionalProperty,
        owl:ObjectProperty ;
    rdfs:label "platform" ;
    dc:description "The Platform used for the acquisition.  If more than one platform is used for creating the product, then the AcquisitionInformation object occurs more than once." ;
    dcterms:source "OGC 17-003"^^xsd:string ;
    rdfs:domain eop:AcquisitionInformation ;
    rdfs:isDefinedBy eop: ;
    rdfs:range eop:Platform .

eop:platformSerialIdentifier a owl:DatatypeProperty ;
    rdfs:label "platformSerialIdentifier" ;
    dcterms:source "OGC 17-003"^^xsd:string ;
    rdfs:comment "Platform serial identifier (e.g. for Seasat : 1)." ;
    rdfs:domain eop:Platform ;
    rdfs:isDefinedBy eop: ;
    rdfs:range xsd:string .

eop:platformShortName a owl:DatatypeProperty ;
    rdfs:label "platformShortName" ;
    dcterms:source "OGC 17-003"^^xsd:string ;
    rdfs:comment "Platform short name (e.g. \"Seasat\" or \"ENVISAT\")." ;
    rdfs:domain eop:Platform ;
    rdfs:isDefinedBy eop: ;
    rdfs:range xsd:string .

eop:polarisationChannels a owl:ObjectProperty ;
    rdfs:label "polarisationChannels" ;
    dcterms:source "OGC 17-003"^^xsd:string ;
    rdfs:comment """Polarisation channel transmit/receive configuration: horizontal, vertical.
Values:
- HH
- HV
- VH
- VV
- HH, VV
- HH, VH
- HH, HV
- VH, VV
- VH, HV
- VV, HV
- VV, VH
- HV, VH
- HH, HV, VH, VV
- UNDEFINED""";
    rdfs:domain eop:AcquisitionParameters ;
    rdfs:isDefinedBy eop: ;
    rdfs:range eop:PolarisationChannelsType .

eop:polarisationMode a owl:ObjectProperty ;
    rdfs:label "polarisationMode" ;
    dcterms:source "OGC 17-003"^^xsd:string ;
    rdfs:comment """Polarisation mode taken from codelist:
S (for single),
D (for dual),
T (for twin),
Q (for quad),
UNDEFINED.""";
    rdfs:domain eop:AcquisitionParameters ;
    rdfs:isDefinedBy eop: ;
    rdfs:range eop:PolarisationModeType .

eop:processingCenter a owl:DatatypeProperty ;
    rdfs:label "processingCenter" ;
    dcterms:source "OGC 17-003"^^xsd:string ;
    rdfs:comment "Processing center code. Possible values are mission specific." ;
    rdfs:domain eop:ProcessingInformation ;
    rdfs:isDefinedBy eop: ;
    rdfs:range xsd:string .

eop:processingDate a owl:DatatypeProperty ;
    rdfs:label "processingDate" ;
    dcterms:source "OGC 17-003"^^xsd:string ;
    rdfs:comment "Processing date time." ;
    rdfs:domain eop:ProcessingInformation ;
    rdfs:isDefinedBy eop: ;
    rdfs:range xsd:dateTime .

eop:processingLevel a owl:DatatypeProperty ;
    rdfs:label "processingLevel" ;
    dcterms:source "OGC 17-003"^^xsd:string ;
    rdfs:comment "Processing level applied to the product: \"1A\", \"1B\", \"1C\", \"2\", \"3\"." ;
    rdfs:domain eop:ProcessingInformation ;
    rdfs:isDefinedBy eop: ;
    rdfs:range xsd:string .

eop:processingMethod a owl:DatatypeProperty ;
    rdfs:label "processingMethod" ;
    dcterms:source "OGC 17-003"^^xsd:string ;
    rdfs:comment "Method used to compute datalayer. (e.g. Kalman filtering, ROSE)." ;
    rdfs:domain eop:ProcessingInformation ;
    rdfs:isDefinedBy eop: ;
    rdfs:range xsd:string .

eop:processingMethodVersion a owl:DatatypeProperty ;
    rdfs:label "processingMethodVersion" ;
    dcterms:source "OGC 17-003"^^xsd:string ;
    rdfs:comment "Method version (e.g. 1.0)." ;
    rdfs:domain eop:ProcessingInformation ;
    rdfs:isDefinedBy eop: ;
    rdfs:range xsd:string .

eop:processingMode a owl:DatatypeProperty ;
    rdfs:label "processingMode" ;
    dcterms:source "OGC 17-003"^^xsd:string ;
    rdfs:comment """Processing mode taken from mission specific code list.
Examples of values are:
•	NRT
•	NOMINAL
•	BACKLOGGED
•	REPROCESSED
•	VALIDATE.""";
    rdfs:domain eop:ProcessingInformation ;
    rdfs:isDefinedBy eop: ;
    rdfs:range xsd:string .

eop:processorName a owl:DatatypeProperty ;
    rdfs:label "processorName" ;
    dcterms:source "OGC 17-003"^^xsd:string ;
    rdfs:comment "Processor software name (e.g. FastROSE)." ;
    rdfs:domain eop:ProcessingInformation ;
    rdfs:isDefinedBy eop: ;
    rdfs:range xsd:string .

eop:processorVersion a owl:DatatypeProperty ;
    rdfs:label "processorName" ;
    dcterms:source "OGC 17-003"^^xsd:string ;
    rdfs:comment "Processor software version (e.g. 1.0)." ;
    rdfs:domain eop:ProcessingInformation ;
    rdfs:isDefinedBy eop: ;
    rdfs:range xsd:string .

eop:productContentType a owl:DatatypeProperty ;
    rdfs:label "productContentType" ;
    dcterms:source "OGC 17-003"^^xsd:string ;
    rdfs:comment """Classification of product according to ground type covered. Note cardinality allows for multiple instances of this property.
Allowed Values:
•	COASTAL
•	CONTINENTAL
•	HYDROLOGY
•	ICE
•	OPEN_OCEAN
•	OTHER
•	REGIONAL.""";
    rdfs:domain eop:ProcessingInformation ;
    rdfs:isDefinedBy eop: ;
    rdfs:range xsd:string .

eop:productGroupId a owl:DatatypeProperty ;
    rdfs:label "productGroupId" ;
    dcterms:source "OGC 17-003"^^xsd:string ;
    rdfs:comment "Holds the identifier of a particular group to which the product belongs to. Group members represent then \"granules\" or \"portions\" of end-user products that are eligible for specific aggregations (e.g. all Sentinel-2 granules having the same productGroupId can be assembled together to form a Sentinel-2 end-user product)." ;
    rdfs:domain eop:ProductInformation ;
    rdfs:isDefinedBy eop: ;
    rdfs:range xsd:string .

eop:productInformation a owl:FunctionalProperty,
        owl:ObjectProperty ;
    rdfs:label "productInformation" ;
    dc:description "Contains product information." ;
    dcterms:source "OGC 17-003"^^xsd:string ;
    rdfs:comment "Contains product information." ;
    rdfs:domain eop:Properties ;
    rdfs:isDefinedBy eop: ;
    rdfs:range eop:ProductInformation .

eop:productType a owl:DatatypeProperty ;
    rdfs:label "productType" ;
    dcterms:source "OGC 17-003"^^xsd:string ;
    rdfs:comment "Describes the product type in case that mixed types are available within a single collection, this is a ground segment specific definition." ;
    rdfs:domain eop:ProductInformation ;
    rdfs:isDefinedBy eop: ;
    rdfs:range xsd:string .

eop:productVersion a owl:DatatypeProperty ;
    rdfs:label "productVersion" ;
    dcterms:source "OGC 17-003"^^xsd:string ;
    rdfs:comment "Product version." ;
    rdfs:domain eop:ProductInformation ;
    rdfs:isDefinedBy eop: ;
    rdfs:range xsd:string .

eop:qualityDegradation a owl:DatatypeProperty ;
    rdfs:label "qualityDegradation" ;
    dcterms:source "OGC 17-003"^^xsd:string ;
    rdfs:comment "Quality degradation percentage (i.e. uom=’%’)." ;
    rdfs:domain eop:QualityInformation ;
    rdfs:isDefinedBy eop: ;
    rdfs:range xsd:double .

eop:qualityDegradationQuotationMode a owl:DatatypeProperty ;
    rdfs:label "qualityDegradationQuotationMode" ;
    dcterms:source "OGC 17-003"^^xsd:string ;
    rdfs:comment """Indicator to know how the quality degradation percentage has been calculated.
Values:
AUTOMATIC, MANUAL.""";
    rdfs:domain eop:QualityInformation ;
    rdfs:isDefinedBy eop: ;
    rdfs:range xsd:string .

eop:qualityDegradationTag a owl:DatatypeProperty ;
    rdfs:label "qualityDegradationTag" ;
    dcterms:source "OGC 17-003"^^xsd:string ;
    rdfs:comment """Contains further textual information concerning the quality degradation.  It shall be provided if qualityStatus value is DEGRADED. Possible values are mission specific and should refer to mission/ground segment dedicated codeSpace.
Example of values could be "RADIOMETRY" or "GEOLOCATION".""";
    rdfs:domain eop:QualityInformation ;
    rdfs:isDefinedBy eop: ;
    rdfs:range xsd:string .

eop:qualityInformation a owl:FunctionalProperty,
        owl:ObjectProperty ;
    rdfs:label "qualityInformation" ;
    dcterms:source "OGC 17-003"^^xsd:string ;
    rdfs:comment "Contains properties related to the quality of the product." ;
    rdfs:domain eop:ProductInformation ;
    rdfs:isDefinedBy eop: ;
    rdfs:range eop:QualityInformation .

eop:qualityStatus a owl:DatatypeProperty ;
    rdfs:label "qualityStatus" ;
    dcterms:source "OGC 17-003"^^xsd:string ;
    rdfs:comment """Indicator that specifies whether the product quality is degraded or not.  This optional field shall be provided if the product has passed a quality check.
Values:
DEGRADED, NOMINAL.""";
    rdfs:domain eop:QualityInformation ;
    rdfs:isDefinedBy eop: ;
    rdfs:range xsd:string .

eop:relativeOrbitNumber a owl:DatatypeProperty ;
    rdfs:label "relativeOrbitNumber" ;
    dcterms:source "OGC 17-003"^^xsd:string ;
    rdfs:comment "Orbit number since start of cycle." ;
    rdfs:domain eop:AcquisitionParameters ;
    rdfs:isDefinedBy eop: ;
    rdfs:range xsd:integer .

eop:resolution a owl:DatatypeProperty ;
    rdfs:label "resolution" ;
    dcterms:source "OGC 17-003"^^xsd:string ;
    rdfs:comment "Sensor resolution.  Unit of measure is SI base unit (m) without prefix." ;
    rdfs:domain eop:AcquisitionParameters ;
    rdfs:isDefinedBy eop: ;
    rdfs:range xsd:double .

eop:roll a owl:DatatypeProperty ;
    rdfs:label "roll" ;
    dcterms:source "OGC 17-003"^^xsd:string ;
    rdfs:comment "Satellite roll angle in degrees (i.e. uom='deg')." ;
    rdfs:domain eop:AcquisitionAngles ;
    rdfs:isDefinedBy eop: ;
    rdfs:range xsd:double .

eop:samplingRate a owl:DatatypeProperty ;
    rdfs:label "samplingRates" ;
    dcterms:source "OGC 17-003"^^xsd:string ;
    rdfs:comment "Rate at which samples are provided in product. Some products may contain more than one sampling rate, e.g. 1kHz and 20kHz. Cardinality is therefore zero to many.  Unit of measure (Hz) is SI derived unit without prefix." ;
    rdfs:domain eop:AcquisitionParameters ;
    rdfs:isDefinedBy eop: ;
    rdfs:range xsd:double .

eop:sensorType a owl:ObjectProperty ;
    rdfs:label "sensorType" ;
    dcterms:source "OGC 17-003"^^xsd:string ;
    rdfs:comment """Sensor type based on codelist.  Values:
       - OPTICAL
       - RADAR
       - ALTIMETRIC
       - ATMOSPHERIC
       - LIMB.""";
    rdfs:domain eop:Instrument ;
    rdfs:isDefinedBy eop: ;
    rdfs:range eop:SensorType .

eop:size a owl:DatatypeProperty ;
    rdfs:label "size" ;
    dcterms:source "OGC 17-003"^^xsd:string ;
    rdfs:comment "Product size (bytes) allowing the user to realise how long a download is likely to take." ;
    rdfs:domain eop:ProductInformation ;
    rdfs:isDefinedBy eop: ;
    rdfs:range xsd:integer .

eop:snowCover a owl:DatatypeProperty ;
    rdfs:label "snowCover" ;
    dcterms:source "OGC 17-003"^^xsd:string ;
    rdfs:comment "Snow cover percentage (i.e. uom=’%’)." ;
    rdfs:domain eop:CoverageDescription ;
    rdfs:isDefinedBy eop: ;
    rdfs:range xsd:double .

eop:spectralRange a owl:ObjectProperty ;
    rdfs:label "spectralRange" ;
    dcterms:source "OGC 17-003"^^xsd:string ;
    rdfs:comment """The observed Spectral Range:
Values:
- INFRARED
- NIR
- SWIR
- MWIR
- LWIR
- FIR
- UV
- VISIBLE
- MICROWAVE
- OTHER.""";
    rdfs:domain eop:WavelengthInformation ;
    rdfs:isDefinedBy eop: ;
    rdfs:range eop:SpectralRangeType .

eop:startTimeFromAscendingNode a owl:DatatypeProperty ;
    rdfs:label "startTimeFromAscendingNode" ;
    dcterms:source "OGC 17-003"^^xsd:string ;
    rdfs:comment "Start time of acquisition in milliseconds from ascending node date." ;
    rdfs:domain eop:AcquisitionParameters ;
    rdfs:isDefinedBy eop: ;
    rdfs:range xsd:integer .

eop:startWavelength a owl:DatatypeProperty ;
    rdfs:label "startWavelength" ;
    dcterms:source "OGC 17-003"^^xsd:string ;
    rdfs:comment "Start of the observed wavelength range.  Unit of measure is SI base unit (m) without prefix." ;
    rdfs:domain eop:WavelengthInformation ;
    rdfs:isDefinedBy eop: ;
    rdfs:range xsd:double .

eop:status a owl:FunctionalProperty,
        owl:ObjectProperty ;
    rdfs:label "status" ;
    dc:description """Refers to product status.
   
Fixed Values :
 - ARCHIVED
 - ACQUIRED
 - CANCELLED
 - FAILED
 - PLANNED
 - POTENTIAL
 - REJECTED
 - QUALITYDEGRADED.""";
    dcterms:source "OGC 17-003"^^xsd:string ;
    rdfs:domain eop:Properties ;
    rdfs:isDefinedBy eop: ;
    rdfs:range eop:StatusType .

eop:statusDetail a owl:DatatypeProperty ;
    rdfs:label "statusDetail" ;
    dcterms:source "OGC 17-003"^^xsd:string ;
    rdfs:comment "This field refers to the status value. It should be used to motivate the reason of a failure, cancelation, rejection or degraded quality." ;
    rdfs:domain eop:ProductInformation ;
    rdfs:isDefinedBy eop: ;
    rdfs:range xsd:string .

eop:statusSubType a owl:DatatypeProperty ;
    rdfs:label "statusSubType" ;
    dcterms:source "OGC 17-003"^^xsd:string ;
    rdfs:comment """Refines the status of a product when the “status” is set to “ARCHIVED”.  
Possible values:
- “ON-LINE”
- “OFF-LINE”.""";
    rdfs:domain eop:ProductInformation ;
    rdfs:isDefinedBy eop: ;
    rdfs:range xsd:string .

eop:swathIdentifier a owl:DatatypeProperty ;
    rdfs:label "swathIdentifier" ;
    dcterms:source "OGC 17-003"^^xsd:string ;
    rdfs:comment "Swath identifier (e.g. Envisat ASAR has 7 distinct swaths (I1,I2,I3...I7) that correspond to precise incidence angles for the sensor)." ;
    rdfs:domain eop:AcquisitionParameters ;
    rdfs:isDefinedBy eop: ;
    rdfs:range xsd:string .

eop:tileId a owl:DatatypeProperty ;
    rdfs:label "tileId" ;
    dcterms:source "OGC 17-003"^^xsd:string ;
    rdfs:comment """While track/frame can be used to represent the first part of an MGRS coordinate (i.g. grid zone), the tileId identifies e.g. the second part of an MGRS coordinate (square identification), e.g. in case of Sentinel.
Used when the world reference system coordinates can not be expressed in X/Y (Track/Frame) terms, such has for UTM tiles. (used for Sentinel-2 L1C granules).""";
    rdfs:domain eop:AcquisitionParameters ;
    rdfs:isDefinedBy eop: ;
    rdfs:range xsd:string .

eop:timeliness a owl:DatatypeProperty ;
    rdfs:label "timeliness" ;
    dcterms:source "OGC 17-003"^^xsd:string ;
    rdfs:comment """Timeliness of the product, such as "near real time", "rush". Possible values are mission specific and shall refer to mission/ground segment dedicated codeSpace.
Example of values could be "NRT", "NOMINAL", “NTC” or “STC”.""";
    rdfs:domain eop:ProductInformation ;
    rdfs:isDefinedBy eop: ;
    rdfs:range xsd:string .

eop:verticalResolution a owl:DatatypeProperty ;
    rdfs:label "verticalResolution" ;
    dcterms:source "OGC 17-003"^^xsd:string ;
    rdfs:comment """lmb: Vertical spacing of data (if regular)
atm: Full width at half maximum of the rows of the vertical averaging kernel matrix
Unit of measure is SI base unit (m) without prefix.""";
    rdfs:domain eop:AcquisitionParameters ;
    rdfs:isDefinedBy eop: ;
    rdfs:range xsd:double .

eop:wavelengthResolution a owl:DatatypeProperty ;
    rdfs:label "wavelengthResolution" ;
    dcterms:source "OGC 17-003"^^xsd:string ;
    rdfs:comment "Spacing between consecutive wavelengths.   Unit of measure is SI base unit (m) without prefix." ;
    rdfs:domain eop:WavelengthInformation ;
    rdfs:isDefinedBy eop: ;
    rdfs:range xsd:double .

eop:wavelengths a owl:ObjectProperty ;
    rdfs:label "wavelengths" ;
    dcterms:source "OGC 17-003"^^xsd:string ;
    rdfs:comment "List of discrete wavelengths observed in the product." ;
    rdfs:domain eop:AcquisitionParameters ;
    rdfs:isDefinedBy eop: ;
    rdfs:range eop:WavelengthInformation .

eop:wrsLatitudeGrid a owl:DatatypeProperty ;
    rdfs:label "wrsLatitudeGrid" ;
    dcterms:source "OGC 17-003"^^xsd:string ;
    rdfs:comment "Neutral wrsLatitudeGrid equivalent to frame in track/frame,  J in K/J, etc." ;
    rdfs:domain eop:AcquisitionParameters ;
    rdfs:isDefinedBy eop: ;
    rdfs:range xsd:string .

eop:wrsLongitudeGrid a owl:DatatypeProperty ;
    rdfs:label "wrsLongitudeGrid" ;
    dcterms:source "OGC 17-003"^^xsd:string ;
    rdfs:comment "Neutral wrsLongitudeGrid equivalent to track in track/frame, K in K/J, etc." ;
    rdfs:domain eop:AcquisitionParameters ;
    rdfs:isDefinedBy eop: ;
    rdfs:range xsd:string .

eop:yaw a owl:DatatypeProperty ;
    rdfs:label "yaw" ;
    dcterms:source "OGC 17-003"^^xsd:string ;
    rdfs:comment "Satellite yaw angle in degrees (i.e. uom='deg')." ;
    rdfs:domain eop:AcquisitionAngles ;
    rdfs:isDefinedBy eop: ;
    rdfs:range xsd:double .

eop:AltitudeUnitType a owl:Class ;
    rdfs:label "AltitudeUnitType" ;
    rdfs:comment "Enumeration of altitudeUnit constants." ;
    rdfs:isDefinedBy eop: ;
    owl:equivalentClass [ a owl:Class ;
            owl:oneOf ( <http://www.opengis.net/ont/eo-geojson/1.0/Unit/Bar> <http://www.opengis.net/ont/eo-geojson/1.0/Unit/Meter> ) ] .

<http://www.opengis.net/ont/eo-geojson/1.0/SpectralRange/FIR> a eop:SpectralRangeType ;
    dc:description "SpectralRange type constant for Far Infrared (FIR)." ;
    skos:broader <http://www.opengis.net/ont/eo-geojson/1.0/SpectralRange/INFRARED> .

<http://www.opengis.net/ont/eo-geojson/1.0/SpectralRange/LWIR> a eop:SpectralRangeType ;
    dc:description "SpectralRange type constant for Long Wavelength Infrared (LWIR)." ;
    skos:broader <http://www.opengis.net/ont/eo-geojson/1.0/SpectralRange/INFRARED> .

<http://www.opengis.net/ont/eo-geojson/1.0/SpectralRange/MWIR> a eop:SpectralRangeType ;
    dc:description "SpectralRange type constant for Mid Wavelength Infrared (MWIR)." ;
    skos:broader <http://www.opengis.net/ont/eo-geojson/1.0/SpectralRange/INFRARED> .

<http://www.opengis.net/ont/eo-geojson/1.0/SpectralRange/NIR> a eop:SpectralRangeType ;
    dc:description "SpectralRange type constant for Near Infrared (NIR)." ;
    skos:broader <http://www.opengis.net/ont/eo-geojson/1.0/SpectralRange/INFRARED> .

<http://www.opengis.net/ont/eo-geojson/1.0/SpectralRange/SWIR> a eop:SpectralRangeType ;
    dc:description "SpectralRange type constant for Short Wavelength Infrared (SWIR)." ;
    skos:broader <http://www.opengis.net/ont/eo-geojson/1.0/SpectralRange/INFRARED> .

eop:TemporalInformation a owl:Class ;
    rdfs:label "TemporalInformation" ;
    dcterms:source "OGC 17-003"^^xsd:string ;
    rdfs:comment "Contains the properties related to the start and end time of the acquisition of the data.  Its properties are inherited by the AcquisitionParameters object." ;
    rdfs:isDefinedBy eop: .

<http://www.opengis.net/ont/eo-geojson/1.0/Unit/Bar> a eop:Unit,
        owl:NamedIndividual ;
    rdfs:label "bar" ;
    dc:description "Unit constant representing non-SI unit \"bar\" (bar)." .

<http://www.opengis.net/ont/eo-geojson/1.0/Unit/Meter> a eop:Unit,
        owl:NamedIndividual ;
    rdfs:label "meter" ;
    dc:description "Unit constant representing SI unit \"meter\" (m)." .

eop:Unit a owl:Class ;
    rdfs:label "Unit" ;
    rdfs:comment "Base class to include all unit constants." ;
    rdfs:isDefinedBy eop: .

eop:AntennaLookDirectionType a owl:Class ;
    rdfs:label "AntennaLookDirectionType" ;
    rdfs:comment "Enumeration of antennaLookDirectionType constants." ;
    rdfs:isDefinedBy eop: .

eop:CoverageDescription a owl:Class ;
    rdfs:label "CoverageDescription" ;
    rdfs:comment "Contains the properties related to the coverage. Its properties are inherited by the ProductInformation object." ;
    rdfs:isDefinedBy eop: .

eop:Instrument a owl:Class ;
    rdfs:label "Instrument" ;
    dcterms:source "OGC 17-003"^^xsd:string ;
    vann:example """
{
    "@context": "https://www.opengis.net/eo-geojson/1.0",
    "type": "Instrument",
    "id":  "http://gcmdservices.gsfc.nasa.gov/kms/concept/a37282d4-322c-4dd0-8edc-36099b9b586c",
    "sensorType": "RADAR", 
    "instrumentShortName": "SAR"
}
   """;
    rdfs:comment "Contains the properties of the instrument that was used to perform the observation.  Use as \"id\" the URI defined by GCMD to identify the instrument.  A list of URI can be downloaded from https://gcmdservices.gsfc.nasa.gov/static/kms/instruments/instruments.rdf." ;
    rdfs:isDefinedBy eop: ;
    rdfs:seeAlso <https://gcmdservices.gsfc.nasa.gov/static/kms/instruments/instruments.rdf> .

eop:MeasurementType a owl:Class ;
    rdfs:label "MeasurementType" ;
    rdfs:comment "Enumeration of measurementType constants." ;
    rdfs:isDefinedBy eop: .

eop:OrbitType a owl:Class ;
    rdfs:label "OrbitType" ;
    rdfs:comment "Enumeration of orbitType constants." ;
    rdfs:isDefinedBy eop: .

eop:Properties a owl:Class ;
    rdfs:label "Properties" ;
    rdfs:comment "Object containing the properties of the Earth Observation." ;
    rdfs:isDefinedBy eop: ;
    rdfs:seeAlso <https://tools.ietf.org/html/rfc7946> ;
    rdfs:subClassOf eop:DataIdentification,
        owc:Properties .

eop:AcquisitionInformation a owl:Class ;
    rdfs:label "AcquisitionInformation" ;
    vann:example """
{
    "@context": "https://www.opengis.net/eo-geojson/1.0",
    "type": "AcquisitionInformation",
    "platform": {
        "id": "http://gcmdservices.gsfc.nasa.gov/kms/concept/1bffe898-f4a2-458e-92c5-cd7c9c1cd5f0",
        "platformShortName": "Seasat", 
        "platformSerialIdentifier": "1"
    }, 
    "instrument": {
        "id":  "http://gcmdservices.gsfc.nasa.gov/kms/concept/a37282d4-322c-4dd0-8edc-36099b9b586c",
        "sensorType": "RADAR", 
        "instrumentShortName": "SAR"
    },  
    "acquisitionParameters": {
        "operationalMode": "IM", 
        "polarisationMode": "S", 
        "polarisationChannels": "HH",
        "beginningDateTime": "1978-09-27T01:04:30Z", 
        "endingDateTime": "1978-09-27T01:04:45Z", 
        "acquisitionType": "NOMINAL", 
        "acquisitionSubType": "DEFAULT", 
        "orbitNumber": "1316", 
        "orbitDirection": "DESCENDING", 
        "antennaLookDirection": "RIGHT", 
        "acquisitionAngles": {
            "minimumIncidenceAngle": 19.6, 
            "maximumIncidenceAngle": 9.6, 
            "incidenceAngleVariation": 9.6
        }
    }
}
   """;
    rdfs:comment "Acquisition information of the Earth Observation as defined in OGC 17-003" ;
    rdfs:isDefinedBy eop: .

eop:AcquisitionType a owl:Class ;
    rdfs:label "AcquisitionType" ;
    rdfs:comment "Enumeration of acquisitionType constants." ;
    rdfs:isDefinedBy eop: .

eop:DataIdentification a owl:Class ;
    rdfs:label "DataIdentification" ;
    dcterms:source "OGC 17-003"^^xsd:string ;
    rdfs:comment "Base class of Properties." ;
    rdfs:isDefinedBy eop: .

eop:OrbitDirectionType a owl:Class ;
    rdfs:label "OrbitDirectionType" ;
    rdfs:comment "Enumeration of orbit direction constants." ;
    rdfs:isDefinedBy eop: .

eop:Platform a owl:Class ;
    rdfs:label "Platform" ;
    dcterms:source "OGC 17-003"^^xsd:string ;
    vann:example """
{
    "@context": "https://www.opengis.net/eo-geojson/1.0",
    "type": "Platform",
    "id": "http://gcmdservices.gsfc.nasa.gov/kms/concept/a1498dff-002d-4d67-9091-16822c608221",
    "platformShortName": "Seasat", 
    "platformSerialIdentifier": "1",
    "orbitType": "LEO"
}
   """;
    rdfs:comment "Contains the properties of the platform (satellite) that was used to perform the observation.  Use as \"id\" the URI defined by GCMD to identify the platform.  A list of URI can be downloaded from https://gcmdservices.gsfc.nasa.gov/static/kms/platforms/platforms.rdf." ;
    rdfs:isDefinedBy eop: ;
    rdfs:seeAlso <https://gcmdservices.gsfc.nasa.gov/static/kms/platforms/platforms.rdf> .

eop:VerticalSpatialDomain a owl:Class ;
    rdfs:label "VerticalSpatialDomain" ;
    dcterms:source "OGC 17-003"^^xsd:string ;
    rdfs:comment "Contains the properties related to the spatial extent in the vertical dimension.  Its properties are inherited by the AcquisitionParameters object." ;
    rdfs:isDefinedBy eop: .

eop:QualityInformation a owl:Class ;
    rdfs:label "QualityInformation" ;
    rdfs:comment "Contains the properties related to the quality of the product." ;
    rdfs:isDefinedBy eop: .

<http://www.opengis.net/ont/eo-geojson/1.0/SpectralRange/INFRARED> a eop:SpectralRangeType ;
    dc:description "SpectralRange type constant." ;
    skos:narrower <http://www.opengis.net/ont/eo-geojson/1.0/SpectralRange/FIR>,
        <http://www.opengis.net/ont/eo-geojson/1.0/SpectralRange/LWIR>,
        <http://www.opengis.net/ont/eo-geojson/1.0/SpectralRange/MWIR>,
        <http://www.opengis.net/ont/eo-geojson/1.0/SpectralRange/NIR>,
        <http://www.opengis.net/ont/eo-geojson/1.0/SpectralRange/SWIR> .

eop:CategoryType a owl:Class ;
    rdfs:label "CategoryType" ;
    rdfs:comment "Enumeration of category constants." ;
    rdfs:isDefinedBy eop: .

eop:PolarisationModeType a owl:Class ;
    rdfs:label "PolarisationModeType" ;
    rdfs:comment "Enumeration of polarisationMode constants." ;
    rdfs:isDefinedBy eop: .

eop:SensorType a owl:Class ;
    rdfs:label "SensorType" ;
    rdfs:comment "Enumeration of sensorType constants." ;
    rdfs:isDefinedBy eop: .

eop:WavelengthInformation a owl:Class ;
    rdfs:label "WavelengthInformation" ;
    dcterms:source "OGC 17-003"^^xsd:string ;
    rdfs:comment "Contains the properties of the instrument related to the wavelengths used for the observation." ;
    rdfs:isDefinedBy eop: .

eop:OrbitParameters a owl:Class ;
    rdfs:label "OrbitParameters" ;
    dcterms:source "OGC 17-003"^^xsd:string ;
    rdfs:comment "Contains the properties related to the orbit.  Its properties are inherited by the AcquisitionParameters object." ;
    rdfs:isDefinedBy eop: .

eop:StatusType a owl:Class ;
    rdfs:label "StatusType" ;
    rdfs:comment "Enumeration of acquisition status constants." ;
    rdfs:isDefinedBy eop: .

eop:ProcessingInformation a owl:Class ;
    rdfs:label "ProcessingInformation" ;
    rdfs:comment "Contains the properties related to the processing of the data." ;
    rdfs:isDefinedBy eop: .

eop:SpectralRangeType a owl:Class ;
    rdfs:label "SpectralRangeType" ;
    rdfs:comment "Enumeration of spectralRangeType constants." ;
    rdfs:isDefinedBy eop: .

eop:ProductInformation a owl:Class ;
    rdfs:label "ProductInformation" ;
    rdfs:comment "Product information of the Earth Observation product as defined in OGC 17-003" ;
    rdfs:isDefinedBy eop: ;
    rdfs:subClassOf eop:CoverageDescription,
        eop:ProcessingInformation .

eop:PolarisationChannelsType a owl:Class ;
    rdfs:label "PolarisationChannelsType" ;
    rdfs:comment "Enumeration of polarisationChannels constants." ;
    rdfs:isDefinedBy eop: .

eop:AcquisitionAngles a owl:Class ;
    rdfs:label "AcquisitionAngles" ;
    vann:example """
{
    "@context": "https://www.opengis.net/eo-geojson/1.0",
    "type": "AcquisitionAngles",
    "minimumIncidenceAngle": 19.6, 
    "maximumIncidenceAngle": 9.6, 
    "incidenceAngleVariation": 9.6
}
   """;
    rdfs:comment "Contains the properties related to the acquisition angles." ;
    rdfs:isDefinedBy eop: .

eop:AcquisitionParameters a owl:Class ;
    rdfs:label "AcquisitionParameters" ;
    dcterms:source "OGC 17-003"^^xsd:string ;
    vann:example """
{
    "@context": "https://www.opengis.net/eo-geojson/1.0",
    "type": "AcquisitionParameters",
    "beginningDateTime": "1978-09-27T01:04:30Z", 
    "endingDateTime": "1978-09-27T01:04:45Z", 
    "acquisitionType": "NOMINAL", 
    "acquisitionSubType": "DEFAULT", 
    "orbitNumber": "1316", 
    "orbitDirection": "DESCENDING", 
    "antennaLookDirection": "RIGHT", 
    "acquisitionAngles": {
        "minimumIncidenceAngle": 19.6, 
        "maximumIncidenceAngle": 9.6, 
        "incidenceAngleVariation": 9.6
    }
}
   """;
    rdfs:comment "Contains the properties related to the acquisition of the data." ;
    rdfs:isDefinedBy eop: ;
    rdfs:subClassOf eop:OrbitParameters,
        eop:TemporalInformation,
        eop:VerticalSpatialDomain .

eop: a owl:Ontology ;
    dc:contributor "John Taylor, CGI"^^xsd:string,
        "Olivier Barois, European Space Agency"^^xsd:string,
        "Sirko Schindler, DLR"^^xsd:string ;
    dc:creator "Yves Coene, Spacebel s.a."^^xsd:string ;
    dc:date "2018-11-09"^^xsd:string ;
    dc:title "OGC 17-003 - Earth Observation Dataset Metadata Vocabulary" ;
    dcterms:license "http://www.opengeospatial.org/ogc/software" ;
    vann:preferredNamespacePrefix "eop" ;
    vann:preferredNamespaceUri "http://www.opengis.net/ont/eo-geojson/1.0/" ;
    void:vocabulary dcterms: ;
    rdfs:comment """This vocabulary defines the classes and properties required to model Earth Observation (EO) metadata for datasets (i.e. products or granules).  It provides the models for the exchange of information describing EO datasets, both within and between different organisations.
        The implementation is derived from the conceptual models defined in the Earth Observation Metadata Profile of Observations and Measurements OGC 10-157r4, and the Unified Metadata Model for Granules (UMM-G)."""^^xsd:string;
    owl:imports <http://geo.spacebel.be/opensearch/owc.owl>,
        <http://purl.org/geojson/vocab#> ;
    owl:versionInfo "1.0.0"^^xsd:string .